theories/aneris_lang/adequacy.v
@@ -8,13 +8,15 @@ Set Default Proof Using "Type".
 
 Import Network.
 
-Theorem adequacy `{anerisPreG Σ Mdl} IPs A s e ip σ φ (ports : gset port)
-  (st0 : Mdl) :
+Theorem adequacy `{anerisPreG Σ Mdl} IPs A B s e ip σ φ (st0 : Mdl) :
   (∀ `{anerisG Mdl Σ}, ⊢ |={⊤}=> ∃ (f : socket_address → socket_interp Σ),
-     fixed A -∗ ([∗ set] a ∈ A, a ⤇ (f a)) -∗
-     ([∗ set] i ∈ IPs, free_ip i) -∗ is_node ip -∗
+     fixed A -∗
+     ([∗ set] a ∈ A, a ⤇ (f a)) -∗
+     ([∗ set] b ∈ B, b ⤳ (∅, ∅)) -∗
+     frag_st st0 -∗
+     ([∗ set] i ∈ IPs, free_ip i) -∗
+     is_node ip -∗
      WP (mkExpr ip e) @ s; ⊤ {{v, ⌜φ v⌝ }}) →
-  ports ≠ ∅ →
   ip ∉ IPs →
   dom (gset ip_address) (state_ports_in_use σ) = IPs →
   (∀ ip, ip ∈ IPs → state_ports_in_use σ !! ip = Some ∅) →
@@ -24,7 +26,7 @@ Theorem adequacy `{anerisPreG Σ Mdl} IPs A s e ip σ φ (ports : gset port)
   state_ms σ = ∅ →
   adequate s (mkExpr ip e) σ (λ v _, φ v).
 Proof.
-  intros Hwp Hps Hipdom Hpiiu Hip Hfixdom Hste Hsce Hmse.
+  intros Hwp Hipdom Hpiiu Hip Hfixdom Hste Hsce Hmse.
   set (δ := @AnerisAuxState Mdl (∅,∅) st0).
   eapply (wp_adequacy _ (@aneris_AS Mdl) _ _ _ _  (δ  : aux_state aneris_AS));
     first apply aneris_AS_valid_state_evolution_finitary.
@@ -34,8 +36,8 @@ Proof.
   iMod (fixed_init A) as (γsif) "#Hsif".
   iMod (free_ips_init IPs) as (γips) "[HIPsCtx HIPs]".
   iMod free_ports_auth_init as (γpiu) "HPiu".
-  iMod (gen_heap_light_init (history_init ip ports)) as (γms) "Hms".
-  iMod (model_init st0) as (γm) "[??]".
+  iMod (messages_ctx_init B) as (γms) "[Hms HB]".
+  iMod (model_init st0) as (γm) "[? Hfrag]".
   set (dg :=
          {|
            aneris_node_gnames_name := γmp;
@@ -63,25 +65,26 @@ Proof.
   { iExists _. eauto. }
   iModIntro.
   iExists  (λ σ δ _, aneris_state_interp σ _ ∗ auth_st _)%I, (λ _, True)%I.
-  iSplitR; last first.
-  iSplitR "Hwp HIPs"; last first.
-  { iSpecialize ("Hwp" with "Hsif Hsa' HIPs Hn").
-    iClear "#". iRevert "Hwp". eauto. }
-  iPoseProof (@aneris_state_interp_init _ _ dg IPs _ _ _ _ _ ports
+  iSplitR; [iApply config_wp_correct|].
+  iSplitR "Hwp HIPs HB Hfrag"; last first.
+  { iApply ("Hwp" with "Hsif Hsa' HB Hfrag HIPs Hn"). }
+  iPoseProof (@aneris_state_interp_init _ _ dg IPs _ _ _ _ _
                 with "[Hmp] [] [Hh] [Hs] [Hms] [] [HM] [] [HIPsCtx] [HPiu] ")
     as "Hsi"; eauto; iFrame.
-  iApply config_wp_correct.
 Qed.
 
 Definition safe e σ := @adequate aneris_lang NotStuck e σ (λ _ _, True).
 
-Theorem adequacy_safe `{anerisPreG Σ Mdl} IPs A e ip σ (ports : gset port)
+Theorem adequacy_safe `{anerisPreG Σ Mdl} IPs A B e ip σ (ports : gset port)
         (st0 : Mdl):
   (∀ `{anerisG Mdl Σ}, ⊢ |={⊤}=> ∃ (f : socket_address → socket_interp Σ),
-     fixed A -∗ ([∗ set] a ∈ A, a ⤇ (f a)) -∗
-     ([∗ set] i ∈ IPs, free_ip i) -∗ is_node ip -∗
+     fixed A -∗
+     ([∗ set] a ∈ A, a ⤇ (f a)) -∗
+     ([∗ set] b ∈ B, b ⤳ (∅, ∅)) -∗
+     frag_st st0 -∗
+     ([∗ set] i ∈ IPs, free_ip i) -∗
+     is_node ip -∗
      WP (mkExpr ip e) {{v, True }}) →
-  ports ≠ ∅ →
   ip ∉ IPs →
   dom (gset ip_address) (state_ports_in_use σ) = IPs →
   (∀ ip, ip ∈ IPs → state_ports_in_use σ !! ip = Some ∅) →
@@ -92,15 +95,16 @@ Theorem adequacy_safe `{anerisPreG Σ Mdl} IPs A e ip σ (ports : gset port)
   safe (mkExpr ip e) σ.
 Proof. by apply adequacy. Qed.
 
-Theorem adequacy_hoare `{anerisPreG Σ Mdl} IPs A e σ φ ip (ports : gset port)
-  (st0 : Mdl) :
+Theorem adequacy_hoare `{anerisPreG Σ Mdl} IPs A B e σ φ ip (st0 : Mdl) :
   (∀ `{anerisG Mdl Σ}, ⊢ ∃ (f : socket_address → socket_interp Σ),
-          {{{ fixed A
-            ∗ ([∗ set] a ∈ A, a ⤇ (f a))
-            ∗ ([∗ set] ip ∈ IPs, free_ip ip) ∗ is_node ip }}}
+          {{{ fixed A ∗
+              ([∗ set] a ∈ A, a ⤇ (f a)) ∗
+              ([∗ set] b ∈ B, b ⤳ (∅, ∅)) ∗
+              frag_st st0 ∗
+              ([∗ set] ip ∈ IPs, free_ip ip) ∗
+              is_node ip }}}
           (mkExpr ip e)
           {{{ v, RET v; ⌜φ v⌝ }}}) →
-  ports ≠ ∅ →
   ip ∉ IPs →
   dom (gset ip_address) (state_ports_in_use σ) = IPs →
   (∀ i, i ∈ IPs → state_ports_in_use σ !! i = Some ∅) →
@@ -110,10 +114,10 @@ Theorem adequacy_hoare `{anerisPreG Σ Mdl} IPs A e σ φ ip (ports : gset port)
   state_ms σ = ∅ →
   adequate NotStuck (mkExpr ip e) σ (λ v _, φ v).
 Proof.
-  intros Hwp ????????.
+  intros Hwp ???????.
   eapply (adequacy _ _ _ _ _ _ _ _ st0); try eauto.
   intros ?. iModIntro.
   iDestruct Hwp as (f) "#Hwp".
-  iExists f. iIntros "????".
+  iExists f. iIntros "??????".
   iApply ("Hwp" with "[$]"); auto.
 Qed.
