theories/aneris_lang/lib/nodepar.v
@@ -20,13 +20,13 @@ Section proof.
     WP ((ip1; e1) ||| (ip2; e2)) @["system"] {{ _, True }}.
   Proof.
     iIntros ([HP1 HP2] [Hn1 Hn2]) "(HΦ1 & HΦ2 & HIP1 & HIP2 & Hwp1 & Hwp2)".
-    wp_apply (aneris_wp_start P1 with "[-]"); [done|done|]. iFrame.
+    wp_apply (aneris_wp_start P1 with "[-]"); [done|]. iFrame.
     iSplitR "HΦ1 Hwp1"; last first.
-    { iNext. iIntros "Hp ?". iApply ("Hwp1" with "HΦ1 Hp"). }
+    { iNext. iIntros "Hp". iApply ("Hwp1" with "HΦ1 Hp"). }
     iNext. simpl.
-    wp_apply (aneris_wp_start with "[-]"); [done|done|]. iFrame.
+    wp_apply (aneris_wp_start with "[-]"); [done|]. iFrame.
     iSplitR "HΦ2 Hwp2"; last first.
-    { iNext. iIntros "Hp ?". iApply ("Hwp2" with "HΦ2 Hp"). }
+    { iNext. iIntros "Hp". iApply ("Hwp2" with "HΦ2 Hp"). }
     iNext. by wp_pures.
   Qed.
 
