theories/aneris_lang/state_interp/messages_history.v
@@ -20,10 +20,8 @@ Definition messages_history := prod message_soup message_soup.
 
 Definition messages_history_map := gmap socket_address messages_history.
 
-
 Implicit Types mh : messages_history_map.
 Implicit Types rt : messages_history.
-
 
 (* The set of all received messages *)
 Definition messages_received mh := collect (λ _ rt, rt.1) mh.
@@ -41,57 +39,12 @@ Lemma elem_of_messages_sent mh :
          ∃ sa rt, mh !! sa = Some rt ∧ m ∈ rt.2.
 Proof. by apply elem_of_collect; eauto. Qed.
 
-
 (** Definitions for the message history *)
 Definition messages_received_sent mh : messages_history :=
   (messages_received mh, messages_sent mh).
 
 (* [m] has been received *)
 Definition message_received m mh := m ∈ (messages_received mh).
-
-(* Initialization of message history from a given set of ports *)
-Definition history_init ip ports :
-  gmap socket_address (message_soup * message_soup) :=
-  gset_to_gmap (∅, ∅) (gset_map (λ p, SocketAddressInet ip p) ports).
-
-Lemma history_init_dom ip ports :
-  ports ≠ ∅ →
-  gset_map
-    ip_of_address
-    (gset_map (λ p : positive, SocketAddressInet ip p) ports) =
-  {[ip]}.
-Proof.
-  induction ports as [| p ports Hp IH] using set_ind_L; first done.
-  intros Hu.
-  destruct (decide (ports = ∅)) as [->| Hports].
-  - rewrite right_id_L.
-    assert (ip = ip_of_address (SocketAddressInet ip p)) as -> by done.
-      by rewrite !gset_map_singleton.
-  - rewrite !gset_map_union. rewrite IH; last done.
-    assert (ip = ip_of_address (SocketAddressInet ip p)) as -> by done.
-    rewrite !gset_map_singleton. set_solver.
-Qed.
-
-Lemma history_init_empty ip ports :
-  ∀ a r t, history_init ip ports !! a = Some (r, t) ↔
-                                             ip_of_address a = ip ∧ port_of_address a ∈ ports ∧ (r,t) = (∅, ∅).
-Proof.
-  intros.
-  split.
-  - intros Hinit.
-    apply lookup_gset_to_gmap_Some in Hinit as (Ha & ->).
-    apply gset_map_correct2 in Ha. set_solver.
-  - intros (<- & Hp & ->).
-    rewrite lookup_gset_to_gmap_Some.
-    split; last done.
-    induction ports using set_ind_L; first done.
-    rewrite gset_map_union.
-    destruct (decide (port_of_address a = x)) as [<- | Hneq].
-    + rewrite gset_map_singleton.
-      apply elem_of_union_l, elem_of_singleton.
-        by destruct a.
-    + apply elem_of_union_r. set_solver.
-Qed.
 
 Lemma gset_to_gmap_singleton (v: message_soup * message_soup)
       (a : socket_address) : gset_to_gmap v {[ a ]} = {[a := v]}.
@@ -100,117 +53,32 @@ Proof.
     by rewrite (gset_to_gmap_union_singleton v a ∅) gset_to_gmap_empty.
 Qed.
 
-Lemma history_init_disj ip ports mh :
-  (∀ p : positive, mh !! SocketAddressInet ip p = None) →
-  history_init ip ports ##ₘ mh.
+Lemma messages_received_init B :
+  messages_received (gset_to_gmap (∅, ∅) B) = ∅.
 Proof.
-  intros Hips.
-  rewrite map_disjoint_spec.
-  intros sa rt rt' Hi Hmh.
-  destruct rt as (r,t).
-  erewrite history_init_empty in Hi.
-  specialize (Hips (port_of_address sa)).
-  destruct Hi as (<- & Hps & ?).
-  assert
-    (sa = SocketAddressInet (ip_of_address sa) (port_of_address sa))
-    as Hsa.
-    by destruct sa.
-    rewrite -Hsa in Hips. by rewrite Hips in Hmh.
-Qed.
-
-Lemma not_elem_of_dom_history ip p
-      (mh : gmap socket_address (message_soup * message_soup)) :
-  ip ∉ gset_map ip_of_address (dom (gset socket_address) mh) →
-  SocketAddressInet ip p ∉ dom (gset socket_address) mh.
-Proof.
-  intros Hip Habs.
-  apply Hip. clear Hip.
-  assert (ip = ip_of_address (SocketAddressInet ip p)) as -> by done.
-  rewrite /gset_map.
-  apply elem_of_list_to_set.
-  apply elem_of_list_fmap_1.
-    by apply elem_of_elements.
-Qed.
-
-Lemma history_init_singleton ip p :
-  history_init ip {[p]} = {[ SocketAddressInet ip p := (∅,∅) ]}.
-Proof. by rewrite /history_init gset_map_singleton gset_to_gmap_singleton. Qed.
-
-Lemma history_init_emptyset ip :
-  history_init ip ∅ = ∅.
-Proof. by rewrite /history_init gset_map_empty gset_to_gmap_empty. Qed.
-
-Lemma history_init_singleton_union ip p ps :
-  p ∉ ps →
-  history_init ip ({[p]} ∪ ps) = history_init ip ps ∪ history_init ip {[p]}.
-Proof.
-  intro Hp.
-  rewrite /history_init.
-  rewrite gset_map_union.
-  rewrite gset_map_singleton.
-  rewrite gset_to_gmap_singleton.
-  rewrite gset_to_gmap_union_singleton.
-  rewrite insert_union_singleton_l.
-  apply map_union_comm.
-  apply map_disjoint_dom_2.
-  rewrite dom_singleton_L.
-  rewrite dom_gset_to_gmap.
-  set_solver.
-Qed.
-
-Lemma history_init_sent ip ports :
-  messages_sent (history_init ip ports) = ∅.
-Proof.
-  rewrite /messages_sent /history_init.
+  rewrite /messages_received.
   apply collect_empty_f.
-  intros k a Hka.
-  erewrite lookup_gset_to_gmap_Some in Hka.
-    by  destruct Hka as (? & <-).
+  intros ? [].
+  rewrite lookup_gset_to_gmap_Some.
+  by intros [? [=]].
 Qed.
 
-Lemma history_init_received ip ports :
-  messages_received (history_init ip ports) = ∅.
+Lemma messages_sent_init B :
+  messages_sent (gset_to_gmap (∅, ∅) B) = ∅.
 Proof.
-  rewrite /messages_received /history_init.
-  apply collect_empty_f.
-  intros k a Hka.
-  erewrite lookup_gset_to_gmap_Some in Hka.
-    by  destruct Hka as (? & <-).
-Qed.
-
-Lemma messages_sent_init ip ports mh :
-  history_init ip ports ##ₘ mh →
-  messages_sent (history_init ip ports ∪ mh) =
-  messages_sent mh.
-Proof.
-  intros Hdisj.
   rewrite /messages_sent.
-  rewrite collect_disjoint_union; last done.
-  erewrite history_init_sent.
-    by rewrite left_id_L.
+  apply collect_empty_f.
+  intros ? [].
+  rewrite lookup_gset_to_gmap_Some.
+  by intros [? [=]].
 Qed.
 
-Lemma message_received_init m ip ports mh :
-  history_init ip ports ##ₘ mh →
-  message_received m mh →
-  message_received m (history_init ip ports ∪ mh).
+Lemma messages_received_sent_init B :
+  messages_received_sent (gset_to_gmap (∅, ∅) B) = (∅, ∅).
 Proof.
-  intros Hdij Hmsg.
-  rewrite /message_received /messages_received.
-  erewrite collect_disjoint_union; last done.
-  set_solver.
-Qed.
-
-Lemma messages_received_init ip ports mh :
-  history_init ip ports ##ₘ mh →
-  messages_received (history_init ip ports ∪ mh) =
-  messages_received mh.
-Proof.
-  intros Hdij.
-  rewrite /message_received /messages_received.
-  erewrite collect_disjoint_union; last done.
-  erewrite history_init_received.
-  set_solver.
+  rewrite /messages_received_sent. f_equal.
+  - apply messages_received_init.
+  - apply messages_sent_init.
 Qed.
 
 Lemma messages_sent_insert a R T mh :
@@ -246,55 +114,53 @@ Proof.
   apply collect_insert.
 Qed.
 
+(* The messages in the logical map mh, that tracks received and transmitted
+   messages, have coherent addresses. *)
+Definition messages_addresses_coh mh :=
+  ∀ a R T, mh !! a = Some (R, T) →
+    (∀ m, m ∈ R → m_destination m = a) ∧ (∀ m, m ∈ T → m_sender m = a).
 
-(* The messages in the logical map mh, that tracks
-     received and transmitted messages, have coherent addresses. *)
-  Definition messages_addresses_coh mh :=
-    ∀ a R T, mh !! a = Some (R, T) →
-             (∀ m, m ∈ R → m_destination m = a) ∧
-             (∀ m, m ∈ T → m_sender m = a).
+Definition messages_received_from_sent_coh mh :=
+  messages_received mh ⊆ messages_sent mh.
 
-  Definition messages_received_from_sent_coh mh :=
-    messages_received mh ⊆ messages_sent mh.
+Definition messages_received_from_sent_coh_aux mh :=
+  ∀ rt m,
+    mh !! (m_destination m) = Some rt →
+    m ∈ rt.1 →
+    ∃ rt', mh !! (m_sender m) = Some rt' ∧ m ∈ rt'.2.
 
-  Definition messages_received_from_sent_coh_aux mh :=
-    ∀ rt m,
-      mh !! (m_destination m) = Some rt →
-      m ∈ rt.1 →
-      ∃ rt', mh !! (m_sender m) = Some rt' ∧ m ∈ rt'.2.
-
-  Lemma messages_received_from_sent_corrolary_coh mh :
-    messages_addresses_coh mh →
-    messages_received_from_sent_coh mh →
-    messages_received_from_sent_coh_aux mh.
-  Proof.
-    intros Hacoh Hrcoh.
-    intros rt m Hrt Hm.
-    assert (m ∈ messages_received mh) as Hmr.
-    { by apply elem_of_collect; eauto. }
-    apply Hrcoh, elem_of_collect in Hmr as (sa & rt' & Hrt' & Hmt).
-    assert (mh !! sa = Some (rt'.1, rt'.2)) as Hgas by by destruct rt'.
-    specialize (Hacoh sa rt'.1  rt'.2 Hgas) as (Hc1 & Hc2).
-    specialize (Hc2 m Hmt). set_solver.
-  Qed.
+Lemma messages_received_from_sent_corrolary_coh mh :
+  messages_addresses_coh mh →
+  messages_received_from_sent_coh mh →
+  messages_received_from_sent_coh_aux mh.
+Proof.
+  intros Hacoh Hrcoh.
+  intros rt m Hrt Hm.
+  assert (m ∈ messages_received mh) as Hmr.
+  { by apply elem_of_collect; eauto. }
+  apply Hrcoh, elem_of_collect in Hmr as (sa & rt' & Hrt' & Hmt).
+  assert (mh !! sa = Some (rt'.1, rt'.2)) as Hgas by by destruct rt'.
+  specialize (Hacoh sa rt'.1  rt'.2 Hgas) as (Hc1 & Hc2).
+  specialize (Hc2 m Hmt). set_solver.
+Qed.
 
 Lemma messages_sent_dijsoint a R T mh :
-    mh !! a = Some (R, T) →
-    messages_addresses_coh mh →
-    T ## messages_sent (delete a mh).
-  Proof.
-    intros Ha Hmcoh.
-    apply elem_of_disjoint.
-    intros m HmT Hms.
-    apply elem_of_collect in Hms as (a' & (R',T') & Ha' & Ht).
-    simplify_map_eq.
-    destruct (Hmcoh a R T Ha) as (_ & HT).
-    specialize (HT m HmT).
-    rewrite -HT in Ha'.
-    destruct (decide (a' = (m_sender m))) as [->|Hneq].
-    - by rewrite lookup_delete in Ha'.
-    - rewrite lookup_delete_ne in Ha'; last done.
+  mh !! a = Some (R, T) →
+  messages_addresses_coh mh →
+  T ## messages_sent (delete a mh).
+Proof.
+  intros Ha Hmcoh.
+  apply elem_of_disjoint.
+  intros m HmT Hms.
+  apply elem_of_collect in Hms as (a' & (R',T') & Ha' & Ht).
+  simplify_map_eq.
+  destruct (Hmcoh a R T Ha) as (_ & HT).
+  specialize (HT m HmT).
+  rewrite -HT in Ha'.
+  destruct (decide (a' = (m_sender m))) as [->|Hneq].
+  - by rewrite lookup_delete in Ha'.
+  - rewrite lookup_delete_ne in Ha'; last done.
     destruct (Hmcoh a' R' T' Ha') as (_ & HT').
     specialize (HT' m Ht).
     done.
-  Qed.
+Qed.
