theories/aneris_lang/state_interp/state_interp_gnames_coh.v
@@ -1,17 +1,6 @@
 From stdpp Require Import fin_maps gmap.
-From iris.bi.lib Require Import fractional.
-From iris.proofmode Require Import tactics.
-From iris.base_logic.lib Require Import saved_prop gen_heap.
-From iris_string_ident Require Import ltac2_string_ident.
-From aneris.program_logic Require Export weakestpre adequacy.
-From aneris.program_logic Require Import ectx_lifting.
-From aneris.lib Require Import gen_heap_light.
-From aneris.aneris_lang Require Import
-     aneris_lang notation network resources.
-From aneris.aneris_lang.state_interp Require Import
-     state_interp_def.
-From aneris.aneris_lang.lib Require Import util.
-
+From aneris.aneris_lang Require Import aneris_lang notation network resources.
+From aneris.aneris_lang.state_interp Require Import state_interp_def.
 From RecordUpdate Require Import RecordSet.
 Set Default Proof Using "Type".
 
@@ -23,60 +12,38 @@ Section state_interpretation.
   Context `{!anerisG Mdl Σ}.
 
   (** gnames_coh *)
-  Lemma gnames_coh_singleton ip γs h Sn mh:
-    gset_map ip_of_address (dom (gset socket_address) mh) = {[ ip ]} →
-    gnames_coh {[ip:=γs]} {[ip:=h]} {[ip:=Sn]} mh.
+  Lemma gnames_coh_singleton ip γs h Sn :
+    gnames_coh {[ip:=γs]} {[ip:=h]} {[ip:=Sn]}.
   Proof. rewrite /gnames_coh !dom_singleton_L //. Qed.
 
-  Lemma gnames_coh_valid γm H S ip Mγ :
+  Lemma gnames_coh_valid γm H S ip :
     H !! ip = None →
-    gnames_coh γm H S Mγ →
+    gnames_coh γm H S →
     γm !! ip = None.
   Proof. rewrite -!not_elem_of_dom => _ [-> _] //. Qed.
 
-  Lemma gnames_coh_alloc_node γm H S ip γn mh ports:
-    ports ≠ ∅ →
-    gnames_coh γm H S mh →
-    gnames_coh (<[ip:=γn]> γm) (<[ip:=∅]> H) (<[ip:=∅]> S)
-               (history_init ip ports ∪ mh).
-  Proof. rewrite /gnames_coh !dom_insert_L.
-         intro Hports.
-         move=> [->] [->] -> //=.
-         split_and!; [ set_solver | set_solver |].
-           by rewrite dom_union_L gset_map_union
-                      dom_gset_to_gmap history_init_dom.
-  Qed.
+  Lemma gnames_coh_alloc_node γm H S ip γn :
+    gnames_coh γm H S →
+    gnames_coh (<[ip:=γn]> γm) (<[ip:=∅]> H) (<[ip:=∅]> S).
+  Proof. rewrite /gnames_coh. set_solver. Qed.
 
-  Lemma gnames_coh_update_heap n γm H S h h' mh:
+  Lemma gnames_coh_update_heap n γm H S h h' :
     H !! n = Some h →
-    gnames_coh γm H S mh →
-    gnames_coh γm (<[n:=h']> H) S mh.
+    gnames_coh γm H S →
+    gnames_coh γm (<[n:=h']> H) S.
   Proof.
     intros ?%elem_of_dom_2 [? ?].
     rewrite /gnames_coh dom_insert_L subseteq_union_1_L //=.
     set_solver.
   Qed.
 
-  Lemma gnames_coh_update_sockets n γm H S Sn Sn' mh :
+  Lemma gnames_coh_update_sockets n γm H S Sn Sn' :
     S !! n = Some Sn →
-    gnames_coh γm H S mh →
-    gnames_coh γm H (<[n:=Sn']> S) mh.
+    gnames_coh γm H S →
+    gnames_coh γm H (<[n:=Sn']> S).
   Proof.
     intros ?%elem_of_dom_2 [? ?].
     rewrite /gnames_coh dom_insert_L subseteq_union_1_L //=.
-    set_solver.
-  Qed.
-
-  Lemma gnames_coh_update_history m a γs H S mh v:
-    m !! ip_of_address a = Some γs →
-    gnames_coh m H S mh →
-    gnames_coh m H S (<[a:=v]> mh).
-  Proof.
-    intros ?%elem_of_dom_2 [? [? Hdmh]].
-    rewrite /gnames_coh dom_insert_L //=.
-    split_and!; eauto.
-    rewrite Hdmh.
-    rewrite gset_map_union gset_map_singleton.
     set_solver.
   Qed.
 
