theories/aneris_lang/state_interp/state_interp_messages_history_coh.v
@@ -55,86 +55,31 @@ Section state_interpretation.
     - by eapply Hrbcoh.
   Qed.
 
-  Ltac mhc_unfold_all :=
+  Local Ltac mhc_unfold_all :=
     rewrite /messages_history_coh /message_soup_coh
             /receive_buffers_coh /messages_addresses_coh
             /messages_received_from_sent_coh.
 
    (** messages_history_coh *)
-  Lemma messages_history_coh_init ip ports :
-    messages_history_coh ∅ {[ip := ∅]} (history_init ip ports).
+  Lemma messages_history_coh_init ip B :
+    messages_history_coh ∅ {[ip := ∅]} (gset_to_gmap (∅, ∅) B).
   Proof.
     mhc_unfold_all. split; first set_solver.
     split; first by intros; simplify_map_eq.
-    split; last by rewrite history_init_received history_init_sent.
-    intros ??? Hg. apply history_init_empty in Hg as (?&?&?); set_solver.
+    split.
+    { intros ???. rewrite lookup_gset_to_gmap_Some.
+      intros [? [= <- <-]]. set_solver. }
+    rewrite messages_received_init messages_sent_init //.
   Qed.
 
-  Lemma messages_history_coh_alloc_node_aux M S mh ip :
+  Lemma messages_history_coh_alloc_node M S mh ip :
     messages_history_coh M S mh →
     messages_history_coh M (<[ip:=∅]> S) mh.
   Proof.
     mhc_unfold_all. intros (?&?&?&?). split; first set_solver.
     split; last set_solver. intros ip0 ???????. ddeq ip ip0; set_solver.
   Qed.
-
-  Lemma messages_history_coh_alloc_node_aux_2 M S mh ip p:
-    history_init ip {[p]} ##ₘ mh →
-    messages_history_coh M S mh →
-    messages_history_coh M S (history_init ip {[p]} ∪ mh).
-  Proof.
-    rewrite history_init_singleton.
-    intros Hdisj Hcoh. rewrite -insert_union_singleton_l.
-    revert Hcoh. mhc_unfold_all.
-    intros (H1 & H2 & H3 & H4).
-    split_and!.
-    - intros m Hm. apply H1 in Hm as (R & T & Hmh & Hmt).
-      destruct (decide ((m_sender m) = (SocketAddressInet ip p))) as [Heq|Hneq].
-      + rewrite Heq. rewrite lookup_insert. rewrite -Heq in Hdisj.
-        decompose_map_disjoint. by rewrite Hdisj in Hmh.
-      + rewrite lookup_insert_ne; last done. set_solver.
-    -  intros ip0 Sn sh skt r m HS HSn Hmr.
-       destruct (decide ((m_sender m) = (SocketAddressInet ip p))) as [Heq|Hneq].
-       + rewrite Heq lookup_insert.
-         specialize (H2 ip0 Sn sh skt r m HS HSn Hmr) as (R & T & Hmh & ?).
-         simplify_map_eq. rewrite Heq in Hmh. by rewrite Hdisj in Hmh.
-       + rewrite lookup_insert_ne; last done. set_solver.
-    -  intros a ???. ddeq a (SocketAddressInet ip p); set_solver.
-    - apply elem_of_subseteq.
-      intros m. rewrite !elem_of_collect. intros (a & RT & Hlk & Hm).
-      ddeq a (SocketAddressInet ip p); first done.
-      assert (m ∈ messages_received mh).
-      { apply elem_of_messages_received. set_solver. }
-      assert (m ∈ messages_sent mh) as Hms by by set_solver.
-      apply elem_of_messages_sent in Hms as (sa & rt & Hrt & Hmrt).
-      exists sa, rt.  ddeq sa (SocketAddressInet ip p); last done.
-      simplify_map_eq.
-  Qed.
-
-  Lemma messages_history_coh_alloc_node M S mh ip ports :
-    history_init ip ports ##ₘ mh →
-    messages_history_coh M S mh →
-    messages_history_coh M (<[ip:=∅]>S) (history_init ip ports ∪ mh).
-  Proof.
-    generalize dependent mh. induction ports as [|p ps Hpp IH] using set_ind_L.
-    - rewrite /history_init gset_map_empty gset_to_gmap_empty.
-      intros mh ?. rewrite left_id_L. apply messages_history_coh_alloc_node_aux.
-    - intros mh'. assert ((history_init ip ({[p]} ∪ ps) ∪ mh') =
-              ((history_init ip ps) ∪ ((history_init ip {[p]}) ∪ mh'))) as ->.
-      { assert ( history_init ip ({[p]} ∪ ps) =
-               history_init ip ps ∪ (history_init ip {[p]})) as ->.
-      { by apply history_init_singleton_union. }
-          by rewrite map_union_assoc. }
-      intros Hdisj Hcoh.
-      rewrite history_init_singleton_union in Hdisj; last done.
-        apply map_disjoint_union_l in Hdisj as [Hd1 Hd2].
-      apply IH; last by apply messages_history_coh_alloc_node_aux_2.
-      apply map_disjoint_union_r. split_and!; eauto.
-      apply map_disjoint_dom_2. rewrite{2} /history_init.
-        rewrite gset_map_singleton gset_to_gmap_singleton dom_singleton_L
-                dom_gset_to_gmap. set_solver.
-  Qed.
-
+  
   Lemma messages_history_coh_socketbind M S Sn mh sh skt a:
     let ip := ip_of_address a in
     S !! ip = Some Sn →
